w64x4/proof/Array4.ec
@@ -2,4 +2,7 @@ require import JArray.
 
 clone export PolyArray as Array4  with op size <- 4.
 
+require import JModel.
+abbrev sbb_64 = subc_64.
+
 
